theories/Common.v
@@ -1,0 +1,80 @@
+Require Import Coq.Bool.Bool
+        Coq.Vectors.Vector.
+
+Ltac injections :=
+  repeat match goal with
+         | [ H : _ = _ |- _ ]
+           => injection H; intros; subst; clear H
+         end.
+
+Ltac find_if_inside :=
+  match goal with
+  | [ |- context[if ?X then _ else _] ] => destruct X
+  | [ H : context[if ?X then _ else _] |- _ ]=> destruct X
+  end.
+
+Ltac split_and :=
+  repeat match goal with
+           H : _ /\ _ |- _ => destruct H
+         end.
+
+Section VectorFacts.
+
+  Lemma vector_nth_replace {A} {k}:
+    forall (i : Fin.t k) (v : Vector.t A k) (a : A),
+      Vector.nth (Vector.replace v i a) i = a.
+  Proof.
+    induction i;
+      intros; pattern v; eapply Vector.caseS'; eauto; intros.
+    simpl; eauto.
+  Qed.
+
+  Lemma vector_nth_replace' {A} {k}:
+    forall (i i0 : Fin.t k) (v : Vector.t A k) (a : A),
+      i <> i0 ->
+      Vector.nth (Vector.replace v i a) i0 = Vector.nth v i0.
+  Proof.
+    induction i0;
+      intros; pattern v; eapply Vector.caseS'; eauto; intros.
+    - simpl; revert v a H h t.
+      pattern i; eapply Fin.caseS'; intros; eauto.
+      congruence.
+    - simpl; revert v a H h t.
+      pattern i; eapply Fin.caseS'; intros; eauto.
+      eapply IHi0; congruence.
+  Qed.
+
+  Lemma vector_replace_nth_id {A} {k}:
+    forall (i : Fin.t k) (v : Vector.t A k),
+      Vector.replace v i (Vector.nth v i) = v.
+  Proof.
+    induction i;
+      intros; pattern v; eapply Vector.caseS'; eauto; intros.
+    simpl; eauto.
+    rewrite IHi; reflexivity.
+  Qed.
+
+  Lemma vector_replace_replace_id {A} {k}:
+    forall (i : Fin.t k) (v : Vector.t A k) (a a' : A),
+      Vector.replace (Vector.replace v i a) i a'  = Vector.replace v i a'.
+  Proof.
+    induction i;
+      intros; pattern v; eapply Vector.caseS'; eauto; intros.
+    simpl; eauto.
+    rewrite IHi; reflexivity.
+  Qed.
+
+  Lemma vector_nth_exists {A} {k} (P : A -> Fin.t k -> Prop):
+    (forall (i : Fin.t k), exists (a : A), P a i) ->
+    exists (v : Vector.t A k), forall (i : Fin.t k), P (Vector.nth v i) i.
+  Proof.
+    induction k; intros.
+    - eexists (Vector.nil _); intros; inversion i.
+    - specialize (IHk (fun a i => P a (Fin.FS i)) (fun i => H (Fin.FS i))); destruct IHk.
+      destruct (H Fin.F1).
+      eexists (Vector.cons _ x0 _ x).
+      intros.
+      pattern i; eapply Fin.caseS'; intros; eauto.
+  Qed.
+
+End VectorFacts.
