theories/HLE.v
@@ -1,0 +1,270 @@
+Require Import
+        Coq.Arith.Arith
+        Coq.micromega.Psatz
+        Coq.Sets.Ensembles
+        Coq.Logic.Classical
+        Coq.Program.Tactics.
+
+Require Import
+        Common
+        Maps
+        FunImp
+        HoareCommon
+        Fixpoints
+        Productive.
+
+Section HLE.
+
+  Reserved Notation "Sigma |- {[ P ]}  c  {[ Q ]}#"
+           (at level 40, c at next level).
+
+  Inductive hle_proof (Sigma : total_map funExSpec)
+    : Assertion -> com -> Assertion -> Prop :=
+  | EH_Skip : forall P,
+      Sigma |- {[P]} SKIP {[P]}#
+  | EH_Asgn : forall Q V a,
+      Sigma |- {[Q[V |-> a]]} V ::= a {[Q]}#
+  | EH_Havoc : forall Q V,
+      Sigma |- {[fun st => exists n : nat, Q[V |-> n] st]} (CHavoc V) {[Q]}#
+  | EH_Seq  : forall P c Q d R,
+      Sigma |- {[P]} c {[Q]}# ->
+      Sigma |- {[Q]} d {[R]}# ->
+      Sigma |- {[P]} c;;d {[R]}#
+  | EH_If : forall P Q b c1 c2,
+      Sigma |- {[fun st => P st /\ bassn b st]} c1 {[Q]}# ->
+      Sigma |- {[fun st => P st /\ ~(bassn b st)]} c2 {[Q]}# ->
+               Sigma |- {[P]} TEST b THEN c1 ELSE c2 FI {[Q]}#
+  | EH_While : forall {A : Type} (R : A -> A -> Prop) M P b c,
+      well_founded R ->
+      (forall (a : A),
+          Sigma |- {[fun st => P st /\ bassn b st /\ M a st]} c {[fun st => P st /\ exists a', M a' st /\ R a' a]}#) ->
+      Sigma |- {[fun st => P st /\ exists a, M a st]} WHILE b DO c END {[fun st => P st /\ ~ (bassn b st)]}#
+  | EH_Consequence  : forall (P Q P' Q' : Assertion) c,
+      Sigma |- {[P']} c {[Q']}# ->
+      (forall st, P st -> P' st) ->
+      (forall st, Q' st -> Q st) ->
+      Sigma |- {[P]} c {[Q]}#
+
+  | EH_Spec : forall Q y f xs,
+      Sigma |- {[fun st =>
+                   exists i,
+                   (exists inits,
+                       exists returns,
+                         (Sigma f).(preEx) (Vector.replace inits i (aseval st xs)) /\
+                         (Sigma f).(postEx) (Vector.replace inits i (aseval st xs))
+                                                         returns) /\
+                   forall inits returns,
+                     (Sigma f).(preEx) (Vector.replace inits i (aseval st xs)) ->
+                     (Sigma f).(postEx) (Vector.replace inits i (aseval st xs))
+                                                        returns ->
+                               Q[y |-> Vector.nth returns i] st]} y :::= f $ xs {[Q]}#
+
+  where "Sigma |- {[ P ]}  c  {[ Q ]}#" := (hle_proof Sigma P c Q) : hoare_spec_scope.
+
+  Definition hle_triple
+             (ESigma : ExEnv)
+             (P : Assertion)
+             (c : com)
+             (Q : Assertion) : Prop :=
+    forall st,
+      P st ->
+      ceval_Ex ESigma c st Q.
+
+  Notation "ESigma |= {[ P ]}  c  {[ Q ]}#" :=
+    (hle_triple ESigma P c Q) (at level 90, c at next level)
+    : hoare_spec_scope.
+
+  Hint Resolve bassn_eval_true bassn_eval_false : hoare.
+  Hint Constructors hle_proof : hoare.
+  Hint Constructors ceval.
+
+  Local Hint Constructors ceval.
+  Local Hint Constructors AppearsIn.
+
+  Hint Constructors ceval_Ex : hoare.
+
+  Theorem hle_proof_sound {Sigma : ExEnv}
+    : forall (P Q : Assertion) c,
+      ex_compatible_env Sigma ->
+      funExSpecs |- {[P]} c {[Q]}# ->
+      forall st,
+        P st ->
+        ceval_Ex {| AllEnv := {| funSigs := @funSigs AllEnv;
+                                   funSpecs := @funSpecs AllEnv;
+                                   funDefs := empty |};
+                      funExSpecs := funExSpecs |} c st Q.
+  Proof.
+    induction 2; intros; eauto.
+    - eapply ceval_Ex_Weaken; try solve [econstructor; eauto].
+      unfold Included, In; intros; inversion H1; subst; eauto.
+    - eapply ceval_Ex_Weaken; try solve [econstructor].
+      unfold Included, In; intros; inversion H1; subst; eauto.
+    - destruct H0.
+      eapply ceval_Ex_Weaken; try solve [econstructor; eauto].
+      instantiate (1 := x).
+      unfold Included, In; intros; inversion H1; subst; eauto.
+    - eapply ceval_Ex_Weaken; try solve [econstructor; eauto].
+      firstorder.
+    - destruct (beval st b) eqn:?.
+      + eapply ceval_Ex_Weaken; try solve [econstructor; eauto].
+        firstorder.
+      + eapply ceval_Ex_Weaken.
+        * eapply ceval_Ex_IfFalse; firstorder eauto.
+          eapply IHhle_proof2; firstorder eauto with hoare.
+          eapply bassn_eval_false; eauto.
+        * firstorder.
+    - destruct H3 as [P_st [a M'] ].
+      revert dependent st.
+      induction a as [a IH] using (well_founded_ind H0). intros.
+      destruct (beval st b) eqn:?.
+      + econstructor; eauto; intros.
+        destruct H3 as [P_st' [a' [M_a' lt_a'] ] ]; eauto.
+      + eapply ceval_Ex_Weaken; eauto using ceval_Ex_WhileFalse.
+        unfold Included, Ensembles.In; intros.
+        inversion H3; subst; intuition.
+        eapply bassn_eval_false; eauto.
+    - eapply ceval_Ex_Weaken; eauto.
+    - destruct H0 as [i [ [inits [returns [? ?] ] ] ? ] ].
+      eapply ceval_Ex_Weaken; eauto.
+      + (*specialize (consistent_Sigma f);
+          destruct consistent_Sigma as [pre_f post_f]. *)
+        eapply ceval_Ex_CallSpec; firstorder eauto.
+        * eapply vector_nth_replace.
+      + unfold Included, Ensembles.In; intros.
+        destruct H3 as [v0 [? [? [? [? ?] ] ] ] ].
+        subst.
+        eapply (H2 v0 x0).
+        rewrite <- H5, vector_replace_nth_id; eauto.
+        rewrite <- H5, vector_replace_nth_id; eauto.
+  Qed.
+
+  Theorem hle_proof_very_sound {Sigma : ExEnv}
+          (Complete_Env : forall f, exists fd,  @funDefs (@AllEnv Sigma) f = Some fd) :
+    forall (P Q : Assertion) c,
+      ex_compatible_env Sigma ->
+      Consistent_Env Sigma ->
+      funExSpecs |- {[P]} c {[Q]}# ->
+      forall st, P st
+                 -> exists st' (exe : (AllEnv) |- st =[c]=> st'), Q st'.
+  Proof.
+    unfold hle_triple; intros.
+    eapply (hle_proof_sound _ _ _ H H1) in H2.
+    eapply productive_strong in H2; eauto.
+    eapply productive_sufficient; eauto.
+  Qed.
+
+  Print Assumptions hle_proof_very_sound.
+
+
+ Lemma Empty_PreCondition :
+    forall Sigma c Q,
+        Sigma |- {[fun _ : state => False]} c {[Q]}#.
+  Proof.
+    induction c.
+    - intros; econstructor; intuition eauto; econstructor.
+    - intros; econstructor; intuition eauto; econstructor.
+    - intros; econstructor; intuition eauto; econstructor.
+    - intros; econstructor.
+      eapply EH_Spec.
+      intros; intuition eauto.
+      eauto.
+    - econstructor; eauto.
+    - econstructor; eauto.
+      + econstructor; intuition eauto.
+      + econstructor; intuition eauto.
+    - intros; econstructor.
+      econstructor.
+      apply lt_wf.
+      econstructor.
+      eapply IHc.
+      instantiate (1 := fun _ _ => False).
+      intros ? [? [? ?] ].
+      apply H.
+      intros.
+      split; try eapply H.
+      intuition.
+      intuition.
+      simpl; intuition eauto.
+      simpl; intuition eauto.
+  Qed.
+
+Section HLEPlus.
+  (* Proof that the EH_SpecK' rule is admissible. *)
+  Inductive hle_proof' (Sigma : total_map funExSpec)
+    : Assertion -> com -> Assertion -> Prop :=
+  | EH_Skip' : forall P,
+      Sigma |- {[P]} SKIP {[P]}#
+  | EH_Asgn' : forall Q V a,
+      Sigma |- {[Q[V |-> a]]} V ::= a {[Q]}#
+  | EH_Havoc' : forall Q V,
+      Sigma |- {[fun st => exists n : nat, Q[V |-> n] st]} (CHavoc V) {[Q]}#
+  | EH_Seq'  : forall P c Q d R,
+      Sigma |- {[P]} c {[Q]}# ->
+      Sigma |- {[Q]} d {[R]}# ->
+      Sigma |- {[P]} c;;d {[R]}#
+  | EH_If' : forall P Q b c1 c2,
+      Sigma |- {[fun st => P st /\ bassn b st]} c1 {[Q]}# ->
+      Sigma |- {[fun st => P st /\ ~(bassn b st)]} c2 {[Q]}# ->
+               Sigma |- {[P]} TEST b THEN c1 ELSE c2 FI {[Q]}#
+  | EH_While' : forall {A : Type} (R : A -> A -> Prop) M P b c,
+      well_founded R ->
+      (forall (a : A),
+          Sigma |- {[fun st => P st /\ bassn b st /\ M a st]} c {[fun st => P st /\ exists a', M a' st /\ R a' a]}#) ->
+      Sigma |- {[fun st => P st /\ exists a, M a st]} WHILE b DO c END {[fun st => P st /\ ~ (bassn b st)]}#
+  | EH_Consequence'  : forall (P Q P' Q' : Assertion) c,
+      Sigma |- {[P']} c {[Q']}# ->
+      (forall st, P st -> P' st) ->
+      (forall st, Q' st -> Q st) ->
+      Sigma |- {[P]} c {[Q]}#
+
+  | EH_Spec' : forall Q y f xs,
+      Sigma |- {[fun st =>
+                   exists i,
+                   (exists inits,
+                       exists returns,
+                         (Sigma f).(preEx) (Vector.replace inits i (aseval st xs)) /\
+                         (Sigma f).(postEx) (Vector.replace inits i (aseval st xs))
+                                                         returns) /\
+                   forall inits returns,
+                     (Sigma f).(preEx) (Vector.replace inits i (aseval st xs)) ->
+                     (Sigma f).(postEx) (Vector.replace inits i (aseval st xs))
+                                                        returns ->
+                               Q[y |-> Vector.nth returns i] st]} y :::= f $ xs {[Q]}#
+  | EH_SpecK'
+    : forall Q y f xs i,
+      Sigma |- {[fun st =>
+                   (exists inits,
+                       exists returns,
+                         (Sigma f).(preEx) (Vector.replace inits i (aseval st xs)) /\
+                         (Sigma f).(postEx) (Vector.replace inits i (aseval st xs))
+                                            returns) /\
+                   forall inits returns,
+                     (Sigma f).(preEx) (Vector.replace inits i (aseval st xs)) ->
+                     (Sigma f).(postEx) (Vector.replace inits i (aseval st xs))
+                                        returns ->
+                     Q[y |-> Vector.nth returns i] st]} y :::= f $ xs {[Q]}#
+  where "Sigma |- {[ P ]}  c  {[ Q ]}#" := (hle_proof' Sigma P c Q) : hoare_spec'_scope.
+
+  Lemma EH_SpecK'_Admissible Sigma :
+    forall P c Q,
+      hle_proof Sigma P c Q <-> hle_proof' Sigma P c Q.
+  Proof.
+    split; induction 1; try solve [econstructor; eauto].
+    - eapply EH_Consequence.
+    eapply EH_Spec.
+    2: eauto.
+    simpl; intros.
+    eexists i; eauto.
+  Qed.
+
+End HLEPlus.
+
+End HLE.
+
+Notation "Sigma |= {[ P ]}  c  {[ Q ]}#" :=
+  (hle_triple Sigma P c Q) (at level 90, c at next level)
+  : hoare_spec_scope.
+
+Notation "Sigma |- {[ P ]}  c  {[ Q ]}#" :=
+  (hle_proof Sigma P c Q) (at level 90, c at next level)
+  : hoare_spec_scope.
