theories/Productive.v
@@ -1,0 +1,396 @@
+Require Import
+        Coq.Arith.Arith
+        Coq.micromega.Psatz
+        Coq.Sets.Ensembles
+        Coq.Logic.Classical
+        Coq.Program.Tactics.
+
+Require Import
+        Common
+        Maps
+        FunImp
+        HoareCommon
+        Fixpoints.
+
+Section existential_Execution.
+
+  (* Formalizing existential executions.
+   *)
+
+  Structure funExSpec : Type :=
+    { (* Number of traces involved in the relational specifications *)
+      k : nat;
+      (* Relational precondition on k initial states *)
+      preEx : Vector.t (list nat) (S k) -> Prop;
+      (* Relational postcondition on k initial states and k return values *)
+      postEx : Vector.t (list nat) (S k) -> Vector.t nat (S k) -> Prop }.
+
+  Class ExEnv : Type :=
+    { AllEnv :> Env;
+      funExSpecs : total_map funExSpec }.
+
+  Local Arguments Singleton [_] _.
+
+  Inductive ceval_Ex (Sigma : ExEnv) : com -> state -> Ensemble state -> Prop :=
+    | ceval_Ex_Skip : forall st,
+        ceval_Ex Sigma SKIP st (Singleton st)
+    | ceval_Havoc_Ass  : forall st x a,
+        ceval_Ex Sigma (CHavoc x) st (Singleton (x !-> a ; st))
+    | ceval_Ex_Ass  : forall st x a,
+        ceval_Ex Sigma (x ::= a) st (Singleton (x !-> (aeval st a) ; st))
+    | ceval_Ex_Seq : forall c1 c2 st Q Q',
+        ceval_Ex Sigma c1 st Q ->
+        (forall st', Q st' -> ceval_Ex Sigma c2 st' Q') ->
+         ceval_Ex Sigma (c1 ;; c2) st Q'
+    | ceval_Ex_IfTrue : forall st Q b c1 c2,
+        beval st b = true ->
+        ceval_Ex Sigma c1 st Q ->
+        ceval_Ex Sigma (TEST b THEN c1 ELSE c2 FI) st Q
+    | ceval_Ex_IfFalse : forall st b c1 c2 Q,
+        beval st b = false ->
+        ceval_Ex Sigma c2 st Q ->
+        ceval_Ex Sigma (TEST b THEN c1 ELSE c2 FI) st Q
+    | ceval_Ex_WhileFalse : forall b st c,
+        beval st b = false ->
+        ceval_Ex Sigma (WHILE b DO c END) st (Singleton st)
+    | ceval_Ex_WhileTrue : forall st b c Q Q',
+        beval st b = true ->
+        ceval_Ex Sigma c st Q ->
+        (forall st', Q st' ->
+                     ceval_Ex Sigma (WHILE b DO c END) st' Q') ->
+        ceval_Ex Sigma (WHILE b DO c END) st Q'
+    | ceval_Ex_CallDef :
+        forall st Q args x f fd,
+          funDefs f = Some fd ->
+          ceval_Ex Sigma (funBody fd) (build_total_map (funArgs fd) (aseval st args) 0) Q
+          -> ceval_Ex Sigma (x :::= f $ args) st
+                        (fun st' => exists st'', Q st'' /\ st' = (x !-> aeval st'' (funRet fd); st))
+    | ceval_Ex_CallSpec : forall st args x f i inits returns,
+        funDefs f = None ->
+        (funExSpecs f).(preEx) inits ->
+        (funExSpecs f).(postEx) inits returns ->
+        Vector.nth inits i = aseval st args ->
+        (*(funSpecs f).(pre) (aseval st args) ->
+        (f unSpecs f).(post) (Vector.nth returns i) (aseval st args) -> *)
+        ceval_Ex Sigma (x :::= f $ args) st
+                   (fun st' => exists inits returns, (funExSpecs f).(postEx) inits returns
+                                                     /\ (funExSpecs f).(preEx) inits
+                                                     /\ Vector.nth inits i = aseval st args
+                               /\ st' = (x !-> Vector.nth returns i; st))
+  | ceval_Ex_Weaken : forall st c Q Q',
+        ceval_Ex Sigma c st Q ->
+        Included state Q Q' ->
+        ceval_Ex Sigma c st Q'.
+
+  (* Existential executions is a *stronger* property than evaluation-- it forces
+     a command to evaluate to a final state regardless of how
+     nondeterministic choices are made. *)
+  Theorem productive_sufficient (Sigma : ExEnv)
+    (Complete_Env : forall f, exists fd,  @funDefs (@AllEnv Sigma) f = Some fd) :
+    forall (c : com) (st : state) (Q : Ensemble state),
+      ceval_Ex Sigma c st Q ->
+      exists st' (exe : (AllEnv) |- st =[c]=> st'), Q st'.
+  Proof.
+    induction 1.
+    - assert (AllEnv |- st =[ SKIP ]=> st) by econstructor.
+      eexists _, H; econstructor.
+    - assert (AllEnv |- st =[ CHavoc x ]=> _) by econstructor.
+      eexists _, H; econstructor.
+    - eassert (AllEnv |- st =[ x ::= a ]=> _) by (econstructor; eauto).
+      eexists _, H; econstructor.
+    - destruct IHceval_Ex as [st' [exe Q_st'] ].
+      specialize (H0 _ Q_st'); destruct (H1 _ Q_st') as [st'' [exe' Q'_st']].
+      assert (AllEnv |- st =[ c1;; c2 ]=> st'') by (econstructor; eauto).
+      eauto.
+    - destruct IHceval_Ex as [st' [exe Q_st'] ].
+      assert (AllEnv |- st =[ TEST b THEN c1 ELSE c2 FI ]=> st') by (econstructor; eauto).
+      eexists _, H1 ; eauto.
+    - destruct IHceval_Ex as [st' [exe Q_st'] ].
+      assert (AllEnv |- st =[ TEST b THEN c1 ELSE c2 FI ]=> st') by (econstructor; eauto).
+      eexists _, H1; eauto.
+    - assert (AllEnv |- st =[ WHILE b DO c END ]=> st) by (econstructor; eauto).
+      eexists _, H0; eauto; econstructor.
+    - destruct IHceval_Ex as [st' [exe Q_st'] ].
+      specialize (H1 _ Q_st'); destruct (H2 _ Q_st') as [st'' [exe' Q'_st']].
+      assert (AllEnv |- st =[ WHILE b DO c END ]=> st'') by (econstructor; eauto).
+      eauto.
+    - destruct IHceval_Ex as [st' [exe Q_st'] ].
+      eassert (AllEnv |- st =[ x :::= f $ args ]=> _) by (eapply (@E_CallDef AllEnv); eauto).
+      eexists _, H1; eauto.
+    - destruct (Complete_Env f) as [fd' H3]; rewrite H3 in H; discriminate.
+    - destruct IHceval_Ex as [st' [exe Q_st'] ]; eexists _, exe; eauto.
+      eapply H0; apply Q_st'.
+  Qed.
+
+
+  (* An existential environment is consistent if all of its existential specifications
+     imply their universal counterparts.  *)
+  Definition Consistent_Env (Sigma : ExEnv) : Prop :=
+    forall f,
+      (forall inits i, (funExSpecs f).(preEx) inits -> (funSpecs f).(pre) (Vector.nth inits i))
+      /\ (forall inits returns i,
+             (funExSpecs f).(postEx) inits returns ->
+             (funSpecs f).(post) (Vector.nth returns i) (Vector.nth inits i)).
+
+  Section Relationalceval_Ex.
+
+  Variables m : nat.
+  Definition Estate := Vector.t state m.
+  Definition Eprogs := Vector.t com m.
+
+  Inductive Relceval_Ex
+            (Sigma : ExEnv)
+    : Estate -> Eprogs -> Ensemble Estate -> Prop :=
+  | RelP_Finish : forall Est Ec,
+      (forall i, Vector.nth Ec i = CSkip)
+      -> Relceval_Ex Sigma Est Ec (Singleton Est)
+
+    | RelP_SkipIntro : forall Est Q Ec Ec' i,
+      (forall i', i <> i' -> Vector.nth Ec i' = Vector.nth Ec' i') ->
+      Vector.nth Ec' i = CSeq (Vector.nth Ec i) CSkip ->
+      Relceval_Ex Sigma Est Ec' Q ->
+      Relceval_Ex Sigma Est Ec Q
+
+  | RelP_Step :
+      forall Est Q (R : Ensemble state) Ec Ec' i c1 c2,
+        (forall i', i <> i' -> Vector.nth Ec i' = Vector.nth Ec' i') ->
+        Vector.nth Ec i = CSeq c1 c2 ->
+        Vector.nth Ec' i = c2 ->
+        ceval_Ex Sigma c1 (Vector.nth Est i) R ->
+        (forall st,
+            R st ->
+            Relceval_Ex Sigma (Vector.replace Est i st) Ec' Q) ->
+        Relceval_Ex Sigma Est Ec Q
+
+  | RelP_Weaken :
+      forall Est Ec Q Q',
+        Relceval_Ex Sigma Est Ec Q ->
+        Included _ Q Q' ->
+        Relceval_Ex Sigma Est Ec Q'.
+
+  Hint Resolve bassn_eval_true bassn_eval_false : hoare.
+  Hint Constructors ceval.
+
+  Theorem Relceval_Ex_sufficient (Sigma : ExEnv)
+          (Complete_Env : forall f, exists fd,  @funDefs (@AllEnv Sigma) f = Some fd)
+  : forall (Est : Estate)
+           (Ec : Eprogs)
+           (Q : Ensemble Estate),
+      Relceval_Ex Sigma Est Ec Q ->
+      exists Est'
+             (exe : forall i, AllEnv |- (Vector.nth Est i) =[Vector.nth Ec i]=> (Vector.nth Est' i)),
+        Q Est'.
+  Proof.
+    induction 1.
+    - exists Est.
+      assert (forall i, AllEnv |- (Vector.nth Est i) =[Vector.nth Ec i]=> (Vector.nth Est i))
+        as exe
+          by (intros; rewrite H; eauto).
+      eexists exe; econstructor.
+    - destruct IHRelceval_Ex as [Est' [exe QEst] ].
+      assert (forall (i' : Fin.t m), AllEnv |- Vector.nth Est i' =[ Vector.nth Ec i' ]=> Vector.nth Est' i')
+        as exe'.
+      { intros; destruct (Fin.eq_dec i i'); subst.
+        + specialize (exe i'); rewrite H0 in exe.
+          inversion exe; subst.
+          inversion H7; subst; eauto.
+        + rewrite H; eauto.
+      }
+      eauto.
+    - eapply productive_sufficient in H2; eauto; destruct H2 as [st' [exe' R_st'] ].
+      destruct (H4 _ R_st') as [Est' [exes' Q_exes'] ].
+      eexists Est'.
+      assert (forall (i' : Fin.t m), AllEnv |- Vector.nth Est i' =[ Vector.nth Ec i' ]=> Vector.nth Est' i'); eauto.
+      { intros; destruct (Fin.eq_dec i i'); subst.
+        + rewrite H0.
+          econstructor; eauto.
+          specialize (exes' i'); rewrite vector_nth_replace in exes'; eauto.
+        + rewrite H; eauto.
+          specialize (exes' i'); rewrite vector_nth_replace' in exes'; eauto.
+      }
+    - destruct IHRelceval_Ex as [Est' [exes' Q_exes'] ].
+      eexists Est', exes'.
+      eapply H0; eauto.
+  Qed.
+
+  End Relationalceval_Ex.
+
+  (* A productive function definition is one that produces at least
+     one behavior allowed by its specifiction. *)
+  Definition productive_funDef (Sigma : ExEnv)
+             (fs : funExSpec)
+             (fd : funDef) : Prop :=
+    forall inits,
+      fs.(preEx) inits ->
+      Relceval_Ex _ Sigma (Vector.map (fun args => build_total_map (fd.(funArgs)) args 0) inits)
+                    (Vector.const fd.(funBody) _)
+                    (fun finals => fs.(postEx) inits (Vector.map (fun st => aeval st fd.(funRet)) finals)).
+
+  (* An environment is productive if all of its function definitions are
+     productive with respect to their specs.  *)
+  Definition ex_compatible_env (Sigma : ExEnv) : Prop :=
+    forall f fd,
+      funDefs f = Some fd ->
+      productive_funDef Sigma (funExSpecs f) fd.
+
+  Lemma productive_empty
+    : forall Sigs Sigma ESigma,
+      ex_compatible_env {| AllEnv := {| funSigs := Sigs; funSpecs := Sigma; funDefs := empty |};
+                        funExSpecs := ESigma |} .
+  Proof.
+    unfold ex_compatible_env; simpl; intros; discriminate.
+  Qed.
+
+  Lemma Relceval_Ex_ceval_Ex
+    : forall
+      (k : nat)
+      (Sigma : ExEnv)
+      (Complete_Env : forall f, exists fd,  @funDefs (@AllEnv Sigma) f = Some fd)
+      (Q : Ensemble (Estate k))
+      (inits : Vector.t state k)
+      (c : Vector.t com k),
+      Relceval_Ex k Sigma inits c Q ->
+      forall i,
+      ceval_Ex Sigma (Vector.nth c i) (Vector.nth inits i)
+                 (fun st => exists finals, Q finals /\ st = Vector.nth finals i).
+  Proof.
+    intros; induction H.
+    - rewrite H; econstructor.
+      + econstructor.
+      + unfold Included, Ensembles.In; intros.
+        inversion H0; subst.
+        eexists; split; eauto.
+        constructor.
+    - destruct (Fin.eq_dec i i0); subst.
+      + rewrite H0 in IHRelceval_Ex.
+        revert IHRelceval_Ex; clear.
+        generalize
+          (Vector.nth Est i0)
+          (fun st : state => exists finals : Estate k0, Q finals /\ st = Vector.nth finals i0).
+        remember (CSeq (Vector.nth Ec i0) SKIP).
+        intros s P H; revert Heqc; induction H; intros; try discriminate.
+        * injection Heqc; intros; subst.
+          econstructor; eauto.
+          unfold Included, Ensembles.In; intros.
+          eapply H0 in H2; revert H2; clear; intro; remember CSkip; induction H2; try discriminate.
+          econstructor.
+          eapply H. eapply IHceval_Ex; eauto.
+        * econstructor; eauto.
+      + rewrite H; eauto.
+    - destruct (Fin.eq_dec i i0); subst.
+      + rewrite H0.
+        econstructor; intros.
+        eauto; intros.
+        eapply H4 in H1.
+        rewrite vector_nth_replace in H1; eauto.
+      + rewrite H; eauto.
+        eapply productive_sufficient in H2; eauto; destruct H2 as [? [? ?] ].
+        erewrite <- (vector_nth_replace' _ _ Est); eauto.
+    - econstructor; eauto.
+      unfold Included, Ensembles.In; intros.
+      destruct H1 as [? [? ?] ].
+      eexists; split; eauto.
+      eapply H0; eauto.
+  Qed.
+
+  (* Key refinement theorem Theorem: executing a program in a
+     compatible environment must result in a final state included in
+     an existential execution. *)
+  Theorem productive_strong (Sigma : ExEnv)
+          (Complete_Env : forall f, exists fd,  @funDefs (@AllEnv Sigma) f = Some fd) :
+    forall (c : com) (st : state) (Q : Ensemble state),
+      ex_compatible_env Sigma ->
+      ceval_Ex {| AllEnv := {|
+                               funSigs := funSigs;
+                               funSpecs := funSpecs;
+                               funDefs := empty |};
+                    funExSpecs := funExSpecs |}
+                 c st Q ->
+      ceval_Ex Sigma c st Q.
+  Proof.
+    induction 2; intros; try (solve [econstructor; eauto]).
+    - simpl in *; rewrite apply_empty in H0; discriminate.
+    - destruct (@funDefs (@AllEnv Sigma) f) eqn: ?.
+      + pose proof (H _ _ Heqo inits H1).
+        destruct f0.
+        eapply ceval_Ex_Weaken.
+        * econstructor; eauto.
+          eapply Relceval_Ex_ceval_Ex with (i := i) in H4.
+          rewrite Vector.const_nth in H4; simpl in *.
+          erewrite VectorSpec.nth_map, H3 in H4; try reflexivity.
+          apply H4.
+          eauto.
+        * unfold Included, Ensembles.In; intros.
+          destruct H5 as [st'' [ [? ?] ?] ]; intuition; simpl in *.
+          eexists _, _.
+          repeat split.
+          -- apply H7.
+          -- try eassumption.
+          -- subst; eauto.
+          -- subst.
+             erewrite Vector.nth_map; try reflexivity.
+      + eapply (@ceval_Ex_CallSpec Sigma); eauto.
+  Qed.
+
+  Theorem Relceval_Ex_strong (Sigma : ExEnv)
+          (Complete_Env : forall f, exists fd,  @funDefs (@AllEnv Sigma) f = Some fd)
+          (m : nat)
+      : forall (Est : Estate m)
+               (Ec : Eprogs m)
+               (Q : Ensemble (Estate m)),
+      ex_compatible_env Sigma ->
+      Relceval_Ex m {| AllEnv := {|
+                                  funSigs := funSigs;
+                                  funSpecs := funSpecs;
+                                  funDefs := empty |};
+                       funExSpecs := funExSpecs |} Est Ec Q ->
+      Relceval_Ex m Sigma Est Ec Q.
+  Proof.
+    induction 2; intros; try (solve [econstructor; eauto]).
+    eapply RelP_Step; eauto using productive_strong.
+  Qed.
+
+  Theorem productive_refine (Sigma : ExEnv)
+          (Complete_Env : forall f, exists fd,  @funDefs (@AllEnv Sigma) f = Some fd) :
+    forall (c : com) (st : state) (Q : Ensemble state),
+      ex_compatible_env Sigma ->
+      ceval_Ex {| AllEnv := {|
+                               funSigs := funSigs;
+                               funSpecs := funSpecs;
+                               funDefs := empty |};
+                    funExSpecs := funExSpecs |}
+                 c st Q ->
+      exists st' (exe : (AllEnv) |- st =[c]=> st'), Q st'.
+  Proof.
+    intros.
+    eapply productive_sufficient; eauto.
+    eapply productive_strong; eauto.
+  Qed.
+
+
+  Local Hint Constructors ceval.
+  Local Hint Constructors AppearsIn.
+
+  Lemma productive_Weaken :
+    forall Sigma c st Q f fd,
+      ~ AppearsIn f c
+      -> (forall (f' : String.string) (fd' : funDef),
+             funDefs f' = Some fd' -> ~ AppearsIn f (funBody fd'))
+      -> ceval_Ex Sigma c st Q
+      -> ceval_Ex {| AllEnv := {| funSigs := funSigs;
+                                    funSpecs := funSpecs;
+                                    funDefs := f |-> fd; funDefs |};
+                       funExSpecs := funExSpecs |} c st Q.
+  Proof.
+    induction 3; simpl; try solve [econstructor; eauto].
+    - econstructor; eauto.
+      simpl; unfold update, t_update; find_if_inside; eauto.
+      destruct H; subst; eauto.
+    - econstructor; eauto.
+      eapply ceval_Ex_CallSpec; eauto.
+      + simpl; unfold update, t_update; find_if_inside; eauto.
+        destruct H; subst; eauto.
+      + unfold Included, In; eauto.
+  Qed.
+
+End existential_Execution.
