theories/RHLE2.v
@@ -1,0 +1,431 @@
+Require Import
+        Coq.Arith.Arith
+        Coq.Sets.Ensembles
+        Coq.micromega.Psatz
+        Coq.Program.Tactics.
+
+Require Import
+        Common
+        Maps
+        FunImp
+        HoareCommon
+        Hoare
+        Productive
+        HLE.
+
+Definition BinAssertion := state -> state -> Prop.
+
+Definition relAssert_implies (P Q : BinAssertion) : Prop :=
+  forall (st : state)
+         (st' : state),
+    P st st' -> Q st st'.
+
+Section RHLE.
+
+  Definition Ustate := state.
+  Definition Estate := state.
+
+  Definition Uprogs := com.
+  Definition Eprogs := com.
+
+  Definition rhle_triple
+             (Sigma : ExEnv)
+             (P : BinAssertion)
+             (Uc : Uprogs)
+             (Ec : Eprogs)
+             (Q : BinAssertion) : Prop :=
+    forall (Ust Ust' : Ustate)
+           (Est : Estate),
+      AllEnv |- Ust =[ Uc ]=> Ust' ->
+      P Ust Est ->
+      exists Est' (exe : AllEnv |- Est =[ Ec ]=> Est'), Q Ust' Est'.
+
+  Notation "Sigma |= {{ P }}  c1 ~# c2  {[ Q ]}" :=
+    (rhle_triple Sigma P c1 c2 Q) (at level 90, c1 at next level, c2 at next level)
+    : hoare_spec_scope.
+
+  Reserved Notation "Sigma , ESigma |- {{ P }}  c1 ~# c2  {[ Q ]}"
+           (at level 40, c1 at next level, c2 at next level).
+
+  Inductive rhle_proof Sigma ESigma
+    : BinAssertion -> Uprogs -> Eprogs -> BinAssertion -> Prop :=
+  | RHE_Skip : forall P Uc Ec,
+      (Uc = CSkip)
+      -> (Ec = CSkip)
+      -> rhle_proof Sigma ESigma P Uc Ec P
+
+  | RHE_SkipIntroL : forall P Q Uc Ec Uc',
+      Uc' = CSeq Uc CSkip ->
+      rhle_proof Sigma ESigma P Uc' Ec Q ->
+      rhle_proof Sigma ESigma P Uc Ec Q
+
+  | RHE_SkipIntroR : forall P Q Uc Ec Ec',
+      Ec' = CSeq Ec CSkip ->
+      rhle_proof Sigma ESigma P Uc Ec' Q ->
+      rhle_proof Sigma ESigma P Uc Ec Q
+
+  | RHE_StepL :
+      forall P Q R Uc Ec Uc' c1 c2,
+        Uc = CSeq c1 c2 ->
+        Uc' = c2 ->
+        (forall Est,
+            hoare_proof Sigma (fun st => P st Est) c1
+                        (fun st => R st Est)) ->
+        rhle_proof Sigma ESigma R Uc' Ec Q ->
+        rhle_proof Sigma ESigma P Uc Ec Q
+
+  | RHE_StepR :
+      forall P Q R Uc Ec Ec' c1 c2,
+        Ec = CSeq c1 c2 ->
+        Ec' = c2 ->
+        (forall Ast,
+            hle_proof ESigma (fun st => P Ast st) c1
+                        (fun st => R Ast st)) ->
+
+        rhle_proof Sigma ESigma R Uc Ec' Q ->
+        rhle_proof Sigma ESigma P Uc Ec Q
+
+  | RHE_StepIfL :
+      forall P Q Uc Ec Uct Uce b ct ce c2,
+        Uc = CSeq (CIf b ct ce) c2 ->
+        Uct = CSeq ct c2 ->
+        Uce = CSeq ce c2 ->
+        rhle_proof Sigma ESigma (fun Ast Est => P Ast Est /\ bassn b Ast) Uct Ec Q ->
+        rhle_proof Sigma ESigma (fun Ast Est => P Ast Est /\ ~ bassn b Ast) Uce Ec Q ->
+        rhle_proof Sigma ESigma P Uc Ec Q
+
+  | RHE_StepIfR :
+      forall P Q Uc Ec Ect Ece b ct ce c2,
+        Ec = CSeq (CIf b ct ce) c2 ->
+        Ect = CSeq ct c2 ->
+        Ece = CSeq ce c2 ->
+        rhle_proof Sigma ESigma (fun Ast Est => P Ast Est /\ bassn b Est) Uc Ect Q ->
+        rhle_proof Sigma ESigma (fun Ast Est => P Ast Est /\ ~ bassn b Est) Uc Ece Q ->
+        rhle_proof Sigma ESigma P Uc Ec Q
+
+  | RHE_StepAll :
+      forall P Q R Uc Ec Uc1 Uc2 Ec1 Ec2,
+        Uc = CSeq Uc1 Uc2 ->
+        Ec = CSeq Ec1 Ec2 ->
+        rhle_proof Sigma ESigma P Uc1 Ec1 R ->
+        rhle_proof Sigma ESigma R Uc2 Ec2 Q ->
+        rhle_proof Sigma ESigma P Uc Ec Q
+
+  | RHE_FuseLoops :
+      forall (Q I : BinAssertion) Uc Ec Ub Uc' Eb Ec',
+        Uc = CWhile Ub Uc' ->
+        Ec = CWhile Eb Ec' ->
+        (forall Ust Est, I Ust Est /\ ~ bassn Ub Ust /\ ~ bassn Eb Est -> Q Ust Est) ->
+        (forall Ust Est, I Ust Est /\ ~ bassn Ub Ust -> ~ bassn Eb Est) ->
+        (forall Ust Est, I Ust Est /\ ~ bassn Eb Est -> ~ bassn Ub Ust) ->
+        rhle_proof Sigma ESigma (fun Ust Est => I Ust Est /\ bassn Ub Ust) Uc' Ec' I ->
+        rhle_proof Sigma ESigma I  Uc Ec Q
+
+  where "Sigma , ESigma |- {{ P }}  c1 ~# c2  {[ Q ]}" := (rhle_proof Sigma ESigma P c1 c2 Q) : hoare_spec_scope.
+
+  Hint Resolve bassn_eval_true bassn_eval_false : hoare.
+  Hint Constructors rhle_proof : hoare.
+  Hint Unfold rhle_triple hoare_triple hle_triple.
+  Hint Constructors ceval.
+
+  Lemma ceval_Ex_single_step' :
+    forall Sigma c' (Est : Productive.Estate 1) Q,
+      Relceval_Ex _ Sigma Est c' Q ->
+      ceval_Ex Sigma (Vector.nth c' Fin.F1) (Vector.nth Est Fin.F1)  (fun Est' => Q (Vector.cons _ Est' _ (Vector.nil _))).
+  Proof.
+    intros.
+    induction H.
+    - specialize (H Fin.F1); simpl in H; subst.
+      rewrite H.
+      econstructor.
+      econstructor.
+      unfold Included, In; intros; inversion H0; subst.
+      pattern Est; eapply Vector.caseS'; simpl; intros.
+      pattern t; eapply Vector.case0; simpl;
+      econstructor.
+    - generalize dependent i; intro i; pattern i; eapply @Fin.caseS' with (n := 0); simpl; intros.
+      + rewrite H0 in IHRelceval_Ex.
+        revert IHRelceval_Ex; clear.
+        remember (Vector.nth Ec Fin.F1;; SKIP)%imp; remember (Vector.nth Est Fin.F1).
+        induction 1; try congruence.
+        * injections.
+          econstructor.
+          eauto.
+          unfold Included, In; intros.
+          eapply H in H1.
+          revert H1; clear; remember CSkip; induction 1; try congruence; eauto.
+          econstructor.
+          eapply H; eapply IHceval_Ex; eauto.
+        * econstructor; eauto.
+      + eapply Fin.case0; eauto.
+    - subst.
+      generalize dependent i; intro i; pattern i; eapply @Fin.caseS' with (n := 0); simpl; intros.
+      + generalize dependent Est; intro; pattern Est; eapply Vector.caseS'; simpl.
+        rewrite H0.
+        econstructor; eauto; intros.
+      + eapply Fin.case0; eauto.
+    - econstructor; eauto.
+      unfold Included, In; intros.
+      eapply H0; eapply H1.
+  Qed.
+
+  Lemma ceval_Ex_single_step :
+    forall Sigma Ec c' (Est : Estate) Q,
+      (forall R, ceval_Ex Sigma c' Est R ->
+                 ceval_Ex Sigma Ec Est R) ->
+      Relceval_Ex _ Sigma (Vector.cons _ Est _ (Vector.nil _)) (Vector.cons _ c' _ (Vector.nil _)) Q ->
+      Relceval_Ex _ Sigma (Vector.cons _ Est _ (Vector.nil _))  (Vector.cons _ Ec _ (Vector.nil _)) Q.
+  Proof.
+    intros.
+    intros; eapply ceval_Ex_single_step' in H0.
+    eapply H in H0.
+    eapply RelP_SkipIntro with (i := Fin.F1) (Ec' := Vector.cons _ (CSeq _ _) _ (Vector.nil _)); simpl; eauto.
+    - intro i'; pattern i'; eapply @Fin.caseS' with (n := 0); simpl; intros.
+      + elimtype False; eapply H1; eauto.
+      + eapply Fin.case0; eauto.
+    - eapply RelP_Step with (i := Fin.F1) (Ec' := Vector.cons _ CSkip _ (Vector.nil _)); simpl; eauto.
+      intro; pattern i'; eapply @Fin.caseS' with (n := 0); simpl; intros.
+      + elimtype False; eapply H1; eauto.
+      + eapply Fin.case0; eauto.
+      + intros; eapply RelP_Weaken.
+        econstructor.
+        * intro i'; pattern i'; eapply @Fin.caseS' with (n := 0); simpl; intros; eauto.
+          eapply Fin.case0; eauto.
+        * unfold Included, In in *; intros; eauto.
+          inversion H2; subst; eauto.
+  Qed.
+
+  Theorem rhle_proof_Relceval_Ex Sigs Sigma ESigma
+    : forall P Uc Ec Q,
+      rhle_proof Sigma ESigma P Uc Ec Q ->
+      forall (Ust Ust' : Ustate)
+             (Est : Estate),
+        ( {| funSigs := Sigs; funSpecs := Sigma; funDefs := empty |}
+            |- Ust =[ Uc ]=> Ust') ->
+        P Ust Est ->
+        Relceval_Ex _ {| AllEnv := {| funSigs := Sigs; funSpecs := Sigma; funDefs := empty |}; funExSpecs := ESigma |} (Vector.cons _ Est _ (Vector.nil _)) (Vector.cons _ Ec _ (Vector.nil _ )) (fun Est => Q Ust' (Vector.hd Est)).
+  Proof.
+    intros ? ? ? ? pf.
+    induction pf; intros Ust Ust' Est exe HP.
+    - subst.
+      eapply RelP_Weaken.
+      + econstructor; eauto.
+        intro; pattern i; eapply @Fin.caseS' with (n := 0).
+        * reflexivity.
+        * eapply Fin.case0.
+      + unfold Included, Ensembles.In; intros Est' Inc_Est'; inversion Inc_Est'; subst; eauto.
+        inversion exe; subst; simpl; eauto.
+    - eapply IHpf in HP; eauto.
+      intros; subst.
+      econstructor; eauto.
+    - eapply IHpf in HP; eauto.
+      eapply RelP_SkipIntro with (i := Fin.F1) (Ec' := Vector.cons _ Ec' _ (Vector.nil _)); eauto.
+      + intro; pattern i'; eapply Fin.caseS'; try congruence.
+        intro; apply Fin.case0; eauto.
+    - subst; inversion exe; subst.
+      eapply IHpf with (Ust := st'); eauto.
+      + eapply (hoare_proof_sound _ _ _ _ _ (H1 Est) _ _ H2); eauto.
+    - specialize (H1 Ust); subst.
+      eapply @hle_proof_sound with (Sigma := {| AllEnv := {| funSigs := _ |} |}) (P := fun Est => P Ust Est) in HP;
+        eauto using productive_empty.
+      eapply RelP_Step with (i := Fin.F1) (Ec' := (Vector.cons _ c2 _ _)); simpl; eauto.
+      + intro; pattern i'; eapply Fin.caseS'; try congruence.
+        intro; apply Fin.case0; eauto.
+      + simpl in *; eauto.
+    - destruct (beval Ust b) eqn: ?.
+      + eapply IHpf1; subst; eauto.
+        inversion exe; subst.
+        inversion H1; subst; try congruence; eauto.
+      + eapply IHpf2; subst; intuition eauto.
+        inversion exe; subst.
+        inversion H1; subst; try congruence; eauto.
+        rewrite bassn_eval_false in Heqb0; tauto.
+    - destruct (beval Est b) eqn: ?.
+      + eapply IHpf1 with (Est := Est) in exe; try tauto.
+        subst.
+        eapply ceval_Ex_single_step with (c' := CSeq ct c2).
+        * revert Heqb0.
+          clear.
+          remember (ct;; c2)%imp; intros.
+          generalize H b ct ce Heqb0 Heqc; clear; intro; induction H; intros; try discriminate.
+          -- injections.
+             econstructor; eauto.
+             revert H Heqb0; clear.
+             econstructor; eauto.
+          -- eapply ceval_Ex_Weaken; eauto.
+        * eauto.
+      + eapply IHpf2 with (Est := Est) in exe; try tauto.
+        subst.
+        eapply ceval_Ex_single_step with (c' := CSeq ce c2).
+        * revert Heqb0.
+          clear.
+          remember (ce;; c2)%imp; intros.
+          generalize H b ct ce Heqb0 Heqc; clear; intro; induction H; intros; try discriminate.
+          -- injections.
+             econstructor; eauto.
+             revert H Heqb0; clear.
+             intros; eapply ceval_Ex_IfFalse; eauto.
+          -- eapply ceval_Ex_Weaken; eauto.
+        * eauto.
+        * intuition eauto using bassn_eval_false.
+          rewrite bassn_eval_false in Heqb0; tauto.
+    - subst; inversion exe; subst; clear exe.
+      specialize (IHpf1 _ _ _ H1 HP).
+      eapply RelP_Step with (i := Fin.F1) (Ec' := Vector.cons _ Ec2 _ _); simpl; eauto.
+      + intro; pattern i'; eapply @Fin.caseS' with (n := 0); try congruence.
+        intro; eapply Fin.case0; eauto.
+      + revert IHpf1; clear.
+        intro.
+        assert (exists Q,
+                   Relceval_Ex 1 {| AllEnv := {| funSigs := Sigs; funSpecs := Sigma; funDefs := empty |}; funExSpecs := ESigma |}
+                               (Vector.cons Estate Est 0 (Vector.nil Estate)) (Vector.cons Eprogs Ec1 0 (Vector.nil Eprogs))
+                               Q /\ Included _ Q (fun Est0 : Productive.Estate 1 => R st' (Vector.hd Est0))).
+        eexists; split; eauto.
+        unfold Included;  eauto.
+        clear IHpf1; destruct H as [Q [? ?] ].
+        remember (Vector.cons Estate Est 0 (Vector.nil Estate));
+          remember (Vector.cons Eprogs Ec1 0 (Vector.nil Eprogs)).
+        generalize H Est Ec1 R Heqt Heqt0 H0; clear; induction 1.
+        * revert H; pattern Ec; eapply Vector.caseS';
+            intros h t; pattern t; eapply VectorDef.case0.
+          pattern Est; eapply Vector.caseS';
+            intros h' t'; pattern t'; eapply VectorDef.case0; clear;
+              intros; injections.
+          specialize (H Fin.F1); simpl in H; rewrite H.
+          econstructor.
+          eapply ceval_Ex_Skip.
+          unfold Included, Ensembles.In; intros Est' Inc_Est'; inversion Inc_Est'; subst; eauto.
+          unfold Included in *.
+          eapply (H0 (Vector.cons _ _ _ _)); unfold In; simpl; econstructor.
+          (*eapply FunctionalExtensionality.equal_f with (x := Vector.cons _ Est' _ (Vector.nil _)) in HeqP.
+          simpl in HeqP; rewrite <- HeqP; constructor.*)
+        * intros; subst.
+          assert  (ceval_Ex
+                    {|
+                    AllEnv := {| funSigs := Sigs; funSpecs := Sigma; funDefs := empty |};
+                    funExSpecs := ESigma |} (Ec1;; SKIP)%imp Est0 (R st')).
+          eapply IHRelceval_Ex; eauto.
+          revert H0; pattern Ec'; eapply Vector.caseS'; intros h t'; pattern t';
+            eapply Vector.case0; pattern i; eapply Fin.caseS'; simpl; intros; subst; eauto.
+          eapply Fin.case0; eauto.
+          revert H3; clear; remember (Ec1;; SKIP)%imp; intro; revert Heqc; induction H3;
+            intros; try discriminate.
+          -- injections; econstructor; eauto.
+             unfold Included, In; intros.
+             eapply H in H1.
+             revert H1; clear.
+             remember CSkip; intro; revert Heqc; induction H1; intros; try discriminate.
+             econstructor.
+             eapply H; eapply IHceval_Ex; eauto.
+          -- econstructor; eauto.
+        * intros; subst.
+          assert (Ec1 = (c1;; Vector.nth Ec' i)%imp).
+          { revert H0; pattern i; eapply Fin.caseS'; simpl; eauto.
+            intro; apply Fin.case0; eauto. }
+          subst.
+          revert H2; pattern i; eapply Fin.caseS'; simpl; intros; eauto.
+          eapply ceval_Ex_Seq.
+          eauto.
+          intros.
+          eapply H4; eauto.
+          pattern i; eapply Fin.caseS'; simpl; intros; eauto.
+          apply Fin.case0; eauto.
+          pattern Ec'; eapply Vector.caseS';
+            intros h t; pattern t; eapply VectorDef.case0.
+          simpl; eauto.
+          apply Fin.case0; eauto.
+        * intros; subst.
+          eapply IHRelceval_Ex; eauto.
+          unfold Included in *; intros; eauto.
+    - clear pf. revert Ec Eb Ec' Est H0 H1 H2 H3 HP IHpf; induction exe; intros; try congruence.
+      eapply RelP_SkipIntro with (i := Fin.F1) (Ec := Vector.cons _ Ec _ _) (Ec' := Vector.cons _ _ _ (Vector.nil _)).
+      + intro i.
+        pattern i; eapply Fin.caseS'; simpl; intros; try discriminate.
+        congruence.
+        eapply Fin.case0; eauto.
+      + simpl; reflexivity.
+      + eapply RelP_Step with (i := Fin.F1) (Ec' := Vector.cons _ CSkip _ _); simpl; eauto.
+        * intro i'.
+          pattern i'; eapply Fin.caseS'; simpl; intros; try discriminate.
+          congruence.
+          eapply Fin.case0; eauto.
+        * rewrite H1.
+          apply ceval_Ex_WhileFalse.
+          apply bassn_eval_false.
+          injections.
+          eapply H3; intuition eauto.
+          eapply bassn_eval_false in H0; intuition.
+        * intros.
+          injections.
+          eapply RelP_Weaken.
+          eapply RelP_Finish.
+          instantiate (1 := Vector.nil _).
+          intro; pattern i; eapply Fin.caseS'; simpl; intros; eauto.
+          apply Fin.case0; eauto.
+          unfold Included, In; intros.
+          eapply H2.
+          inversion H; subst; simpl.
+          inversion H5; subst; intuition.
+          apply bassn_eval_false in H0; intuition.
+          eapply H3; intuition eauto.
+          apply bassn_eval_false in H0; intuition.
+      + eapply ceval_Ex_single_step with (c' := CSeq Ec' (CWhile Eb Ec')).
+        * subst.
+          assert (beval Est Eb = true).
+          { destruct (beval Est Eb) eqn: ?; eauto.
+            injections.
+            eapply bassn_eval_false in Heqb0.
+            elimtype False; eapply H4; intuition eauto. }
+            intuition.
+            remember (Ec';; WHILE Eb DO Ec' END)%imp.
+          revert Heqc0 H1 R H6; clear;
+          intros Heqc0 H1 R H'; revert Heqc0 H1.
+          induction H'; intros; try congruence; injections.
+          -- econstructor; eauto.
+          -- eapply ceval_Ex_Weaken; eauto.
+        * eapply RelP_Step with (i := Fin.F1) (Ec' := Vector.cons _ (CWhile Eb Ec') _ _) (R := I st'); simpl; eauto.
+          -- intro i'; pattern i'; eapply Fin.caseS'; simpl; intros; try congruence.
+             apply Fin.case0; eauto.
+          -- injections.
+             intuition.
+             assert (I st Est /\ bassn Ub st) by intuition.
+             specialize (IHpf _ _ _ exe1 H1).
+             eapply ceval_Ex_single_step' in IHpf.
+             simpl in IHpf.
+             eapply ceval_Ex_Weaken.
+             eauto.
+             unfold Included, In; intros; intuition.
+  Qed.
+
+  Theorem rhle_proof_refine
+          {Sigma : ExEnv}
+          (Complete_Env : forall f, exists fd,  @funDefs (@AllEnv Sigma) f = Some fd)
+    : forall (P : BinAssertion)
+             (Uc : Uprogs)
+             (Ec : Eprogs)
+             (Q : BinAssertion),
+      ex_compatible_env Sigma ->
+      compatible_env (@AllEnv Sigma) ->
+      rhle_proof (@funSpecs (@AllEnv Sigma)) funExSpecs P Uc Ec Q ->
+      Sigma |= {{P}} Uc ~# Ec {[Q]}.
+  Proof.
+    unfold rhle_triple; intros.
+    eapply (rhle_proof_Relceval_Ex funSigs _ _ _ _ _ _ H1) in H3;
+      eauto using compatible_Env_refine.
+    eapply Relceval_Ex_strong in H3; eauto.
+    eapply Relceval_Ex_sufficient in H3; eauto.
+    destruct H3 as [? [? ?] ]; eauto.
+    specialize (x0 Fin.F1); simpl in *; eauto.
+    eexists _; eexists x0; eauto.
+    revert H3; pattern x; apply Vector.caseS'; simpl; eauto.
+  Qed.
+
+End RHLE.
+
+Notation "Sigma |= {{ P }}  c1 ~# c2  {[ Q ]}" :=
+  (rhle_triple Sigma P c1 c2 Q) (at level 90, c1 at next level, c2 at next level)
+  : hoare_spec_scope.
+
+Notation "Sigma |- {{ P }}  c1 ~# c2  {[ Q ]}" :=
+  (rhle_proof Sigma P c1 c2 Q) (at level 90, c1 at next level, c2 at next level)
+  : hoare_spec_scope.
