theories/README.md
@@ -1,0 +1,8 @@
+* This directory contains a coq formalization of the program logics in the paper.
+* Run make to build everything.
+* Coq 8.9.1 is required; although other versions may work as well.
+
+Theorems from paper can be found in:
+- Theorem B.1: safe_Env_refine in FunImp.v
+- Theorem B.2: productive_refine: Productive.v
+- Theorem B.3 [RHLE is Sound]: rhle_proof_refine in RHLE.v
